Add lemmas

src/Syntax.v
@@ -374,14 +374,14 @@ Module Syntax (P : PAT).
         TmConDef (Kopen_d j X d) (Kopen_ty j X ty) T (Kopen_t (S j) X t')
     end.
 
-  Definition Kclose (X : var) (j : nat) (T : tname) :=
-    match T with
-    | BTName _ => T
-    | FTName Y => If X = Y then BTName j else T
+  Definition Kclose (X : var) (j : nat) (K : con) :=
+    match K with
+    | BCon _ => K
+    | FCon Y => If X = Y then BCon j else K
     end.
 
   Definition Kclose_d (X : var) (j : nat) (d : data) : data :=
-    LibList.map (fun '(T, Ks) => (Kclose X j T, Ks)) d.
+    LibList.map (fun '(T, Ks) => (T, LibList.map (Kclose X j) Ks)) d.
 
   Definition Kclose_k (X : var) (j : nat) (k : kind) :=
     match k with
@@ -395,7 +395,7 @@ Module Syntax (P : PAT).
     | TyFVar Y => T
     | TyArr T1 T2 => TyArr (Kclose_ty X j T1) (Kclose_ty X j T2)
     | TyAll k T' => TyAll (Kclose_k X j k) (Kclose_ty X j T')
-    | TyCon ty T => TyCon (Kclose_ty X j ty) (Kclose X j T)
+    | TyCon ty T => TyCon (Kclose_ty X j ty) T
     | TyData d => TyData (Kclose_d X j d)
     end.
 
@@ -407,10 +407,10 @@ Module Syntax (P : PAT).
     | TmApp t1 t2 => TmApp (Kclose_t X j t1) (Kclose_t X j t2)
     | TmTyLam k t' => TmTyLam (Kclose_k X j k) (Kclose_t X j t')
     | TmTyApp t' T => TmTyApp (Kclose_t X j t') (Kclose_ty X j T)
-    | TmCon K ty t' => TmCon K (Kclose_ty X j ty) (Kclose_t X j t')
-    | TmType t' => TmType (Kclose_t X (S j) t')
+    | TmCon K ty t' => TmCon (Kclose X j K) (Kclose_ty X j ty) (Kclose_t X j t')
+    | TmType t' => TmType (Kclose_t X j t')
     | TmConDef d ty T t' =>
-        TmConDef (Kclose_d X j d) (Kclose_ty X j ty) (Kclose X j T) (Kclose_t X j t')
+        TmConDef (Kclose_d X j d) (Kclose_ty X j ty) T (Kclose_t X (S j) t')
     end.
 
 
@@ -1349,13 +1349,52 @@ Module Syntax (P : PAT).
     introv Hlc. gen n i. solve_eq t. apply* Topen_t_lc.
   Qed.
 
+  Lemma Tclose_d_fresh :
+    forall T i d,
+      T \notin Tfv_d d ->
+      Tclose_d T i d = d.
+  Proof.
+    introv Hfv. unfolds Tclose_d. unfolds Tfv_d.
+    induction~ d.
+    rew_listx in *. destruct a. rewrite~ IHd. destruct t ; solve_var.
+  Qed.
+
+  Lemma Tclose_k_fresh :
+    forall T i k,
+      T \notin Tfv_k k ->
+      Tclose_k T i k = k.
+  Proof. introv Hfv. solve_eq k ; apply~ Tclose_d_fresh. Qed.
+
+  Lemma Tclose_ty_fresh :
+    forall T i ty,
+      T \notin Tfv_ty ty ->
+      Tclose_ty T i ty = ty.
+  Proof.
+    introv Hfv. solve_eq ty.
+    - apply~ Tclose_k_fresh.
+    - destruct t ; solve_var.
+    - apply~ Tclose_d_fresh.
+  Qed.
+
+  Lemma Tclose_t_fresh :
+    forall T i t,
+      T \notin Tfv_t t ->
+      Tclose_t T i t = t.
+  Proof.
+    introv Hfv. gen i. solve_eq t ;
+      try solve [ apply~ Tclose_d_fresh
+                | apply~ Tclose_k_fresh
+                | apply~ Tclose_ty_fresh ].
+    destruct t0 ; solve_var.
+  Qed.
+
   Lemma Tclose_t_open_comm :
     forall i n T v t,
       T \notin Tfv_t v ->
       Tclose_t T i ([n ~> v] t) = [n ~> v] (Tclose_t T i t).
   Proof.
-    introv. gen i n. solve_eq t. admit. (* apply* Tclose_t_fresh. *)
-  Admitted.
+    introv. gen i n. solve_eq t ; apply* Tclose_t_fresh.
+  Qed.
 
   Lemma Topen_ty_topen_comm :
     forall i n T ty1 ty2,
@@ -1378,8 +1417,8 @@ Module Syntax (P : PAT).
       T \notin Tfv_ty ty1 ->
       Tclose_ty T i ({n ~> ty1} ty2) = {n ~> ty1} (Tclose_ty T i ty2).
   Proof.
-    introv. gen n. solve_eq ty2. (* apply* Tclose_ty_fresh. *)
-  Admitted.
+    introv. gen n. solve_eq ty2 ; apply* Tclose_ty_fresh.
+  Qed.
 
   Lemma Tclose_t_topen_comm :
     forall i n T ty t,
@@ -1389,28 +1428,158 @@ Module Syntax (P : PAT).
     introv. gen n i. solve_eq t ; apply* Tclose_ty_topen_comm.
   Qed.
 
+  Lemma Topen_d_Topen_comm :
+    forall i j T T' d,
+      i <> j ->
+      Topen_d i (FTName T) (Topen_d j (FTName T') d) =
+        Topen_d j (FTName T') (Topen_d i (FTName T) d).
+  Proof.
+    introv Hneq. unfolds Topen_d.
+    induction~ d. destruct a. rew_listx. rewrite~ IHd.
+    destruct t ; solve_var.
+  Qed.
+
+  Lemma Topen_k_Topen_comm :
+    forall i j T T' k,
+      i <> j ->
+      Topen_k i (FTName T) (Topen_k j (FTName T') k) =
+        Topen_k j (FTName T') (Topen_k i (FTName T) k).
+  Proof. introv Hneq. solve_eq k ; apply~ Topen_d_Topen_comm. Qed.
+
+  Lemma Topen_ty_Topen_comm :
+    forall i j T T' ty,
+      i <> j ->
+      Topen_ty i (FTName T) (Topen_ty j (FTName T') ty) =
+        Topen_ty j (FTName T') (Topen_ty i (FTName T) ty).
+  Proof.
+    introv Hneq. solve_eq ty.
+    - apply~ Topen_k_Topen_comm.
+    - destruct t ; solve_var.
+    - apply~ Topen_d_Topen_comm.
+  Qed.
+
   Lemma Topen_t_Topen_comm :
     forall i j T T' t,
       i <> j ->
-      Topen_t i T (Topen_t j T' t) = Topen_t j T' (Topen_t i T t).
-  Admitted.
+      Topen_t i (FTName T) (Topen_t j (FTName T') t) =
+        Topen_t j (FTName T') (Topen_t i (FTName T) t).
+  Proof.
+    introv Hneq. gen i j. solve_eq t ;
+      try solve [ apply~ Topen_d_Topen_comm
+                | apply~ Topen_k_Topen_comm
+                | apply~ Topen_ty_Topen_comm ].
+    destruct t0 ; solve_var.
+  Qed.
+
+  Lemma Topen_d_Tclose_comm :
+    forall i j T T' d,
+      i <> j ->
+      T <> T' ->
+      Topen_d i (FTName T) (Tclose_d T' j d) =
+        Tclose_d T' j (Topen_d i (FTName T) d).
+  Proof.
+    introv Hneq1 Hneq2. unfolds Topen_d. unfolds Tclose_d.
+    induction~ d. destruct a. rew_listx. rewrite~ IHd.
+    destruct t ; solve_var.
+  Qed.
+
+  Lemma Topen_k_Tclose_comm :
+    forall i j T T' k,
+      i <> j ->
+      T <> T' ->
+      Topen_k i (FTName T) (Tclose_k T' j k) =
+        Tclose_k T' j (Topen_k i (FTName T) k).
+  Proof. intros. solve_eq k ; apply~ Topen_d_Tclose_comm. Qed.
+
+  Lemma Topen_ty_Tclose_comm :
+    forall i j T T' ty,
+      i <> j ->
+      T <> T' ->
+      Topen_ty i (FTName T) (Tclose_ty T' j ty) =
+        Tclose_ty T' j (Topen_ty i (FTName T) ty).
+  Proof.
+    introv Hneq1 Hneq2. solve_eq ty.
+    - apply~ Topen_k_Tclose_comm.
+    - destruct t ; solve_var.
+    - apply~ Topen_d_Tclose_comm.
+  Qed.
 
   Lemma Topen_t_Tclose_comm :
     forall i j T T' t,
       i <> j ->
       T <> T' ->
       Topen_t i (FTName T) (Tclose_t T' j t) = Tclose_t T' j (Topen_t i (FTName T) t).
-  Admitted.
+  Proof.
+    introv Hneq1 Hneq2. gen i j. solve_eq t ;
+      try solve [ apply~ Topen_d_Tclose_comm
+                | apply~ Topen_k_Tclose_comm
+                | apply~ Topen_ty_Tclose_comm ].
+    destruct t0 ; solve_var.
+  Qed.
+
+  Lemma Kopen_d_Topen_comm :
+    forall i j K T d,
+      Kopen_d i K (Topen_d j T d) = Topen_d j T (Kopen_d i K d).
+  Proof.
+    intros. unfolds Topen_d. unfolds Kopen_d.
+    induction~ d. destruct a. rew_listx. rewrite~ IHd.
+  Qed.
+
+  Lemma Kopen_k_Topen_comm :
+    forall i j K T k,
+      Kopen_k i K (Topen_k j T k) = Topen_k j T (Kopen_k i K k).
+  Proof. intros. solve_eq k ; apply~ Kopen_d_Topen_comm. Qed.
+
+  Lemma Kopen_ty_Topen_comm :
+    forall i j K T ty,
+      Kopen_ty i K (Topen_ty j T ty) = Topen_ty j T (Kopen_ty i K ty).
+  Proof.
+    intros. solve_eq ty.
+    - apply~ Kopen_k_Topen_comm.
+    - apply~ Kopen_d_Topen_comm.
+  Qed.
 
   Lemma Kopen_t_Topen_comm :
     forall i j K T t,
       Kopen_t i K (Topen_t j T t) = Topen_t j T (Kopen_t i K t).
-  Admitted.
+  Proof.
+    intros. gen i j. solve_eq t ;
+      try solve [ apply~ Kopen_d_Topen_comm
+                | apply~ Kopen_k_Topen_comm
+                | apply~ Kopen_ty_Topen_comm ].
+  Qed.
+
+  Lemma Kopen_d_Tclose_comm :
+    forall i j K T d,
+      Kopen_d i K (Tclose_d T j d) = Tclose_d T j (Kopen_d i K d).
+  Proof.
+    intros. unfolds Tclose_d. unfolds Kopen_d.
+    induction~ d. destruct a. rew_listx. rewrite~ IHd.
+  Qed.
+
+  Lemma Kopen_k_Tclose_comm :
+    forall i j K T k,
+      Kopen_k i K (Tclose_k T j k) = Tclose_k T j (Kopen_k i K k).
+  Proof. intros. solve_eq k ; apply~ Kopen_d_Tclose_comm. Qed.
+
+  Lemma Kopen_ty_Tclose_comm :
+    forall i j K T ty,
+      Kopen_ty i K (Tclose_ty T j ty) = Tclose_ty T j (Kopen_ty i K ty).
+  Proof.
+    intros. solve_eq ty.
+    - apply~ Kopen_k_Tclose_comm.
+    - apply~ Kopen_d_Tclose_comm.
+  Qed.
 
   Lemma Kopen_t_Tclose_comm :
     forall i j K T t,
       Kopen_t i K (Tclose_t T j t) = Tclose_t T j (Kopen_t i K t).
-  Admitted.
+  Proof.
+    intros. gen i j. solve_eq t ;
+      try solve [ apply~ Kopen_d_Tclose_comm
+                | apply~ Kopen_k_Tclose_comm
+                | apply~ Kopen_ty_Tclose_comm ].
+  Qed.
 
   Lemma open_inj :
     forall i x t1 t2,
@@ -1419,15 +1588,8 @@ Module Syntax (P : PAT).
       t1 = t2.
   Proof.
     introv Hfv Heq. gen i t2.
-    solve_eq t1 ; destruct t2 ; inverts Heq ; solve_var.
-    - inverts~ H0. notin_false.
-    - rewrite~ (IHt1 (S i) t2).
-    - rewrite~ (IHt1_1 i t2_1). rewrite~ (IHt1_2 i t2_2).
-    - rewrite~ (IHt1 i t2).
-    - rewrite~ (IHt1 i t2).
-    - rewrite~ (IHt1 i t2).
-    - rewrite~ (IHt1 i t2).
-    - rewrite~ (IHt1 i t4).
+    solve_eq t1 ; destruct t2 ; inverts Heq ; solve_var ; fequals*.
+    - inverts H0. notin_false.
   Qed.
 
   Lemma topen_inj :
@@ -1436,7 +1598,10 @@ Module Syntax (P : PAT).
       {i ~> TyFVar x} ty1 = {i ~> TyFVar x} ty2 ->
       ty1 = ty2.
   Proof.
-  Admitted.
+    introv Hfv Heq. gen i ty2.
+    solve_eq ty1 ; destruct ty2 ; inverts Heq ; solve_var ; fequals*.
+    - inverts H0. notin_false.
+  Qed.
 
   Lemma topen_t_inj :
     forall i x t1 t2,
@@ -1444,7 +1609,48 @@ Module Syntax (P : PAT).
       [{i ~> TyFVar x}] t1 = [{i ~> TyFVar x}] t2 ->
       t1 = t2.
   Proof.
-  Admitted.
+    introv Hfv Heq. gen i t2.
+    solve_eq t1 ; destruct t2 ; inverts Heq ; solve_var ; fequals* ;
+      rewrite_all notin_union in Hfv ; apply* topen_inj.
+  Qed.
+
+  Lemma Topen_d_inj :
+    forall i X d1 d2,
+      X \notin Tfv_d d1 \u Tfv_d d2 ->
+      Topen_d i (FTName X) d1 = Topen_d i (FTName X) d2 ->
+      d1 = d2.
+  Proof.
+    introv. gen d2. unfolds Topen_d. unfolds Tfv_d.
+    induction d1 ; introv Hfv Heq ; destruct d2 ; inverts~ Heq.
+    destruct a ; destruct p ; rew_listx in *. rewrite~ (IHd1 d2).
+    do 2 fequals. inverts H0.
+    destruct t ; destruct t0 ; solve_var ; inverts H2 ; notin_false.
+  Qed.
+
+  Lemma Topen_k_inj :
+    forall i X k1 k2,
+      X \notin Tfv_k k1 \u Tfv_k k2 ->
+      Topen_k i (FTName X) k1 = Topen_k i (FTName X) k2 ->
+      k1 = k2.
+  Proof.
+    introv Hfv Heq. gen k2.
+    solve_eq k1 ; destruct k2 ; inverts Heq ; fequals ; apply* Topen_d_inj.
+  Qed.
+
+  Lemma Topen_ty_inj :
+    forall i X ty1 ty2,
+      X \notin Tfv_ty ty1 \u Tfv_ty ty2 ->
+      Topen_ty i (FTName X) ty1 = Topen_ty i (FTName X) ty2 ->
+      ty1 = ty2.
+  Proof.
+    introv Hfv Heq. gen i ty2.
+    solve_eq ty1 ; destruct ty2 ; inverts Heq ; solve_var ; fequals* ;
+      rewrite_all notin_union in Hfv.
+    - apply* Topen_k_inj.
+    - destruct Hfv as ((?&Hfv1)&(?&Hfv2)).
+      destruct t ; destruct t0 ; solve_var ; inverts H1 ; notin_false.
+    - apply* Topen_d_inj.
+  Qed.
 
   Lemma Topen_t_inj :
     forall i X t1 t2,
@@ -1452,7 +1658,53 @@ Module Syntax (P : PAT).
       Topen_t i (FTName X) t1 = Topen_t i (FTName X) t2 ->
       t1 = t2.
   Proof.
-  Admitted.
+    introv Hfv Heq. gen i t2.
+    solve_eq t1 ; destruct t2 ; inverts Heq ; solve_var ; fequals* ;
+      rewrite_all notin_union in Hfv ;
+      try solve [ apply* Topen_d_inj
+                | apply* Topen_k_inj
+                | apply* Topen_ty_inj ].
+    destruct Hfv as ((?&?&Hfv1&?)&(?&?&Hfv2&?)).
+    destruct t0 ; destruct t3 ; solve_var ; inverts H2 ; notin_false.
+  Qed.
+
+  Lemma Kopen_d_inj :
+    forall i X d1 d2,
+      X \notin Kfv_d d1 \u Kfv_d d2 ->
+      Kopen_d i (FCon X) d1 = Kopen_d i (FCon X) d2 ->
+      d1 = d2.
+  Proof.
+    introv. gen d2. unfolds Kopen_d. unfolds Kfv_d.
+    induction d1 ; introv Hfv Heq ; destruct d2 ; inverts~ Heq.
+    destruct a ; destruct p ; rew_listx in *.
+    fequals~. fequals. inverts H0.
+    gen l0. induction l ; introv Hfv Heq ; destruct l0 ; inverts~ Heq.
+    rew_listx in *. fequals~.
+    destruct a ; destruct c ; solve_var ; inverts H0 ; notin_false.
+  Qed.
+
+  Lemma Kopen_k_inj :
+    forall i X k1 k2,
+      X \notin Kfv_k k1 \u Kfv_k k2 ->
+      Kopen_k i (FCon X) k1 = Kopen_k i (FCon X) k2 ->
+      k1 = k2.
+  Proof.
+    introv Hfv Heq. gen k2.
+    solve_eq k1 ; destruct k2 ; inverts Heq ; fequals ; apply* Kopen_d_inj.
+  Qed.
+
+  Lemma Kopen_ty_inj :
+    forall i X ty1 ty2,
+      X \notin Kfv_ty ty1 \u Kfv_ty ty2 ->
+      Kopen_ty i (FCon X) ty1 = Kopen_ty i (FCon X) ty2 ->
+      ty1 = ty2.
+  Proof.
+    introv Hfv Heq. gen i ty2.
+    solve_eq ty1 ; destruct ty2 ; inverts Heq ; solve_var ; fequals* ;
+      rewrite_all notin_union in Hfv.
+    - apply* Kopen_k_inj.
+    - apply* Kopen_d_inj.
+  Qed.
 
   Lemma Kopen_t_inj :
     forall i X t1 t2,
@@ -1460,28 +1712,45 @@ Module Syntax (P : PAT).
       Kopen_t i (FCon X) t1 = Kopen_t i (FCon X) t2 ->
       t1 = t2.
   Proof.
-  Admitted.
+    introv Hfv Heq. gen i t2.
+    solve_eq t1 ; destruct t2 ; inverts Heq ; solve_var ; fequals* ;
+      rewrite_all notin_union in Hfv ;
+      try solve [ apply* Kopen_d_inj
+                | apply* Kopen_k_inj
+                | apply* Kopen_ty_inj ].
+    destruct Hfv as ((Hfv1&?&?)&(Hfv2&?&?)).
+    destruct c ; destruct c0 ; solve_var ; inverts H0 ; notin_false.
+  Qed.
 
   Lemma Topen_d_Tclose :
     forall i T d,
       lcd d ->
       Topen_d i (FTName T) (Tclose_d T i d) = d.
   Proof.
-  Admitted.
+    introv Hlc. unfolds lcd. unfolds Topen_d. unfolds Tclose_d.
+    induction~ Hlc. rew_listx. destruct x. do 2 fequals.
+    destruct H as (HlcT&?).
+    destruct t ; solve_var ; inverts HlcT ; discriminate.
+  Qed.
 
   Lemma Topen_k_Tclose :
     forall i T k,
       lck k ->
       Topen_k i (FTName T) (Tclose_k T i k) = k.
-  Proof.
-  Admitted.
+  Proof. introv Hlc. solve_eq Hlc. apply~ Topen_d_Tclose. Qed.
 
   Lemma Topen_ty_Tclose :
     forall i T ty,
       lct ty ->
       Topen_ty i (FTName T) (Tclose_ty T i ty) = ty.
   Proof.
-  Admitted.
+    introv Hlc. solve_eq Hlc.
+    - apply~ Topen_k_Tclose.
+    - remember (Topen_ty i (FTName T) (Tclose_ty T i T0)).
+      pick_fresh X ; substs. applys~ topen_inj 0 X.
+      rewrite* <- Topen_ty_topen_comm. rewrite* <- Tclose_ty_topen_comm. simpls~.
+    - apply~ Topen_d_Tclose.
+  Qed.
 
   Lemma Topen_t_Tclose :
     forall i T t,
@@ -1513,13 +1782,23 @@ Module Syntax (P : PAT).
   Qed.
 
   Lemma Tclose_d_notin : forall T i d, T \notin Tfv_d (Tclose_d T i d).
-  Admitted.
+  Proof.
+    intros. unfolds Tclose_d. unfolds Tfv_d.
+    induction d ; rew_listx~. destruct a. rewrite notin_union. splits~.
+    destruct t ; solve_var.
+  Qed.
 
   Lemma Tclose_k_notin : forall T i k, T \notin Tfv_k (Tclose_k T i k).
-  Admitted.
+  Proof. intros. induction k ; simpls~. apply~ Tclose_d_notin. Qed.
 
   Lemma Tclose_ty_notin : forall T i ty, T \notin Tfv_ty (Tclose_ty T i ty).
-  Admitted.
+  Proof.
+    intros.
+    induction ty ; intros ; solve_var ; rewrite_all notin_union ; try split~.
+    - apply~ Tclose_k_notin.
+    - destruct t ; solve_var.
+    - apply~ Tclose_d_notin.
+  Qed.
 
   Lemma Tclose_t_notin : forall T i t, T \notin Tfv_t (Tclose_t T i t).
   Proof.
@@ -1531,14 +1810,303 @@ Module Syntax (P : PAT).
     destruct t0 ; solve_var.
   Qed.
 
+  Lemma Kopen_t_open_comm :
+    forall i n K v t,
+      lc v ->
+      Kopen_t i K ([n ~> v] t) = [n ~> v] (Kopen_t i K t).
+  Proof.
+    introv Hlc. gen n i. solve_eq t. apply* Kopen_t_lc.
+  Qed.
+
+  Lemma Kclose_d_fresh :
+    forall K i d,
+      K \notin Kfv_d d ->
+      Kclose_d K i d = d.
+  Proof.
+    introv Hfv. unfolds Kclose_d. unfolds Kfv_d.
+    induction~ d.
+    rew_listx in *. destruct a. do 2 fequals~.
+    induction~ l. rew_listx in *. fequals~.
+    destruct a ; solve_var.
+  Qed.
+
+  Lemma Kclose_k_fresh :
+    forall K i k,
+      K \notin Kfv_k k ->
+      Kclose_k K i k = k.
+  Proof. introv Hfv. solve_eq k ; apply~ Kclose_d_fresh. Qed.
+
+  Lemma Kclose_ty_fresh :
+    forall K i ty,
+      K \notin Kfv_ty ty ->
+      Kclose_ty K i ty = ty.
+  Proof.
+    introv Hfv. solve_eq ty.
+    - apply~ Kclose_k_fresh.
+    - apply~ Kclose_d_fresh.
+  Qed.
+
+  Lemma Kclose_t_fresh :
+    forall K i t,
+      K \notin Kfv_t t ->
+      Kclose_t K i t = t.
+  Proof.
+    introv Hfv. gen i. solve_eq t ;
+      try solve [ apply~ Kclose_d_fresh
+                | apply~ Kclose_k_fresh
+                | apply~ Kclose_ty_fresh ].
+    destruct c ; solve_var.
+  Qed.
+
+  Lemma Kclose_t_open_comm :
+    forall i n K v t,
+      K \notin Kfv_t v ->
+      Kclose_t K i ([n ~> v] t) = [n ~> v] (Kclose_t K i t).
+  Proof.
+    introv. gen i n. solve_eq t ; apply* Kclose_t_fresh.
+  Qed.
+
+  Lemma Kopen_ty_topen_comm :
+    forall i n K ty1 ty2,
+      lct ty1 ->
+      Kopen_ty i K ({n ~> ty1} ty2) = {n ~> ty1} (Kopen_ty i K ty2).
+  Proof.
+    introv. gen n. solve_eq ty2. apply* Kopen_ty_lct.
+  Qed.
+
+  Lemma Kopen_t_topen_comm :
+    forall i n K ty t,
+      lct ty ->
+      Kopen_t i K ([{n ~> ty}] t) = [{n ~> ty}] (Kopen_t i K t).
+  Proof.
+    introv. gen n i. solve_eq t ; apply* Kopen_ty_topen_comm.
+  Qed.
+
+  Lemma Kclose_ty_topen_comm :
+    forall i n K ty1 ty2,
+      K \notin Kfv_ty ty1 ->
+      Kclose_ty K i ({n ~> ty1} ty2) = {n ~> ty1} (Kclose_ty K i ty2).
+  Proof.
+    introv. gen n. solve_eq ty2 ; apply* Kclose_ty_fresh.
+  Qed.
+
+  Lemma Kclose_t_topen_comm :
+    forall i n K ty t,
+      K \notin Kfv_ty ty ->
+      Kclose_t K i ([{n ~> ty}] t) = [{n ~> ty}] (Kclose_t K i t).
+  Proof.
+    introv. gen n i. solve_eq t ; apply* Kclose_ty_topen_comm.
+  Qed.
+
+  Lemma Kopen_d_Kopen_comm :
+    forall i j K K' d,
+      i <> j ->
+      Kopen_d i (FCon K) (Kopen_d j (FCon K') d) =
+        Kopen_d j (FCon K') (Kopen_d i (FCon K) d).
+  Proof.
+    introv Hneq. unfolds Kopen_d.
+    induction~ d. destruct a. rew_listx. do 2 fequals~.
+    induction~ l. rew_listx. fequals~.
+    destruct a ; solve_var.
+  Qed.
+
+  Lemma Kopen_k_Kopen_comm :
+    forall i j K K' k,
+      i <> j ->
+      Kopen_k i (FCon K) (Kopen_k j (FCon K') k) =
+        Kopen_k j (FCon K') (Kopen_k i (FCon K) k).
+  Proof. introv Hneq. solve_eq k ; apply~ Kopen_d_Kopen_comm. Qed.
+
+  Lemma Kopen_ty_Kopen_comm :
+    forall i j K K' ty,
+      i <> j ->
+      Kopen_ty i (FCon K) (Kopen_ty j (FCon K') ty) =
+        Kopen_ty j (FCon K') (Kopen_ty i (FCon K) ty).
+  Proof.
+    introv Hneq. solve_eq ty.
+    - apply~ Kopen_k_Kopen_comm.
+    - apply~ Kopen_d_Kopen_comm.
+  Qed.
+
+  Lemma Kopen_t_Kopen_comm :
+    forall i j K K' t,
+      i <> j ->
+      Kopen_t i (FCon K) (Kopen_t j (FCon K') t) =
+        Kopen_t j (FCon K') (Kopen_t i (FCon K) t).
+  Proof.
+    introv Hneq. gen i j. solve_eq t ;
+      try solve [ apply~ Kopen_d_Kopen_comm
+                | apply~ Kopen_k_Kopen_comm
+                | apply~ Kopen_ty_Kopen_comm ].
+    destruct c ; solve_var.
+  Qed.
+
+  Lemma Kopen_d_Kclose_comm :
+    forall i j K K' d,
+      i <> j ->
+      K <> K' ->
+      Kopen_d i (FCon K) (Kclose_d K' j d) =
+        Kclose_d K' j (Kopen_d i (FCon K) d).
+  Proof.
+    introv Hneq1 Hneq2. unfolds Kopen_d. unfolds Kclose_d.
+    induction~ d. destruct a. rew_listx. do 2 fequals~.
+    induction~ l. rew_listx. fequals~.
+    destruct a ; solve_var.
+  Qed.
+
+  Lemma Kopen_k_Kclose_comm :
+    forall i j K K' k,
+      i <> j ->
+      K <> K' ->
+      Kopen_k i (FCon K) (Kclose_k K' j k) =
+        Kclose_k K' j (Kopen_k i (FCon K) k).
+  Proof. intros. solve_eq k ; apply~ Kopen_d_Kclose_comm. Qed.
+
+  Lemma Kopen_ty_Kclose_comm :
+    forall i j K K' ty,
+      i <> j ->
+      K <> K' ->
+      Kopen_ty i (FCon K) (Kclose_ty K' j ty) =
+        Kclose_ty K' j (Kopen_ty i (FCon K) ty).
+  Proof.
+    introv Hneq1 Hneq2. solve_eq ty.
+    - apply~ Kopen_k_Kclose_comm.
+    - apply~ Kopen_d_Kclose_comm.
+  Qed.
+
+  Lemma Kopen_t_Kclose_comm :
+    forall i j K K' t,
+      i <> j ->
+      K <> K' ->
+      Kopen_t i (FCon K) (Kclose_t K' j t) = Kclose_t K' j (Kopen_t i (FCon K) t).
+  Proof.
+    introv Hneq1 Hneq2. gen i j. solve_eq t ;
+      try solve [ apply~ Kopen_d_Kclose_comm
+                | apply~ Kopen_k_Kclose_comm
+                | apply~ Kopen_ty_Kclose_comm ].
+    destruct c ; solve_var.
+  Qed.
+
+  Lemma Kopen_d_Kclose :
+    forall i K d,
+      lcd d ->
+      Kopen_d i (FCon K) (Kclose_d K i d) = d.
+  Proof.
+    introv Hlc. unfolds lcd. unfolds Kopen_d. unfolds Kclose_d.
+    induction~ Hlc. rew_listx. destruct x. do 2 fequals.
+    destruct H as (?&HlcK).
+    induction~ l0. rew_listx in *. fequals*. destruct HlcK as (HlcK'&?).
+    destruct a ; solve_var ; inverts HlcK' ; discriminate.
+  Qed.
+
+  Lemma Kopen_k_Kclose :
+    forall i K k,
+      lck k ->
+      Kopen_k i (FCon K) (Kclose_k K i k) = k.
+  Proof. introv Hlc. solve_eq Hlc. apply~ Kopen_d_Kclose. Qed.
+
+  Lemma Kopen_ty_Kclose :
+    forall i K ty,
+      lct ty ->
+      Kopen_ty i (FCon K) (Kclose_ty K i ty) = ty.
+  Proof.
+    introv Hlc. solve_eq Hlc.
+    - apply~ Kopen_k_Kclose.
+    - remember (Kopen_ty i (FCon K) (Kclose_ty K i T)).
+      pick_fresh X ; substs. applys~ topen_inj 0 X.
+      rewrite* <- Kopen_ty_topen_comm. rewrite* <- Kclose_ty_topen_comm. simpls~.
+    - apply~ Kopen_d_Kclose.
+  Qed.
+
+  Lemma Topen_d_Kclose_comm :
+    forall i j K T d,
+      Topen_d i T (Kclose_d K j d) = Kclose_d K j (Topen_d i T d).
+  Proof.
+    intros. unfolds Kclose_d. unfolds Topen_d.
+    induction~ d. destruct a. rew_listx. fequals~.
+  Qed.
+
+  Lemma Topen_k_Kclose_comm :
+    forall i j K T k,
+      Topen_k i T (Kclose_k K j k) = Kclose_k K j (Topen_k i T k).
+  Proof. intros. solve_eq k ; apply~ Topen_d_Kclose_comm. Qed.
+
+  Lemma Topen_ty_Kclose_comm :
+    forall i j K T ty,
+      Topen_ty i T (Kclose_ty K j ty) = Kclose_ty K j (Topen_ty i T ty).
+  Proof.
+    intros. solve_eq ty.
+    - apply~ Topen_k_Kclose_comm.
+    - apply~ Topen_d_Kclose_comm.
+  Qed.
+
+  Lemma Topen_t_Kclose_comm :
+    forall i j K T t,
+      Topen_t i T (Kclose_t K j t) = Kclose_t K j (Topen_t i T t).
+  Proof.
+    intros. gen i j. solve_eq t ;
+      try solve [ apply~ Topen_d_Kclose_comm
+                | apply~ Topen_k_Kclose_comm
+                | apply~ Topen_ty_Kclose_comm ].
+  Qed.
+
   Lemma Kopen_t_Kclose :
     forall i K t,
       lc t ->
       Kopen_t i (FCon K) (Kclose_t K i t) = t.
-  Proof. Admitted.
+  Proof.
+    introv Hlc. gen i.
+    induction Hlc ; intros ; simpls ; fequals* ;
+      try solve [ apply~ Kopen_d_Kclose
+                | apply~ Kopen_k_Kclose
+                | apply~ Kopen_ty_Kclose ].
+    - remember (Kopen_t i (FCon K) (Kclose_t K i t)).
+      pick_fresh x ; substs. applys~ open_inj 0 x.
+      rewrite* <- Kopen_t_open_comm. rewrite* <- Kclose_t_open_comm. simpls~.
+    - remember (Kopen_t i (FCon K) (Kclose_t K i t)).
+      pick_fresh x ; substs. applys~ topen_t_inj 0 x.
+      rewrite* <- Kopen_t_topen_comm. rewrite* <- Kclose_t_topen_comm. simpls~.
+    - solve_var.
+    - remember (Kopen_t i (FCon K) (Kclose_t K i t)).
+      pick_fresh X ; substs. applys~ Topen_t_inj 0 X.
+      rewrite~ <- Kopen_t_Topen_comm. rewrite~ Topen_t_Kclose_comm.
+    - remember (Kopen_ty i (FCon K) (Kclose_ty K i ty)).
+      pick_fresh X ; substs. applys~ topen_inj 0 X.
+      rewrite* <- Kopen_ty_topen_comm. rewrite~ <- Kclose_ty_topen_comm ; simpls~.
+      apply* Kopen_ty_Kclose.
+    - remember (Kopen_t (S i) (FCon K) (Kclose_t K (S i) t)).
+      pick_fresh X ; substs. applys~ Kopen_t_inj 0 X.
+      rewrite~ Kopen_t_Kopen_comm. rewrite~ Kopen_t_Kclose_comm.
+  Qed.
+
+  Lemma Kclose_d_notin : forall K i d, K \notin Kfv_d (Kclose_d K i d).
+  Proof.
+    intros. unfolds Kclose_d. unfolds Kfv_d.
+    induction d ; rew_listx~. destruct a. rewrite notin_union. splits~.
+    induction l ; rew_listx~.
+    rewrite notin_union. splits~. destruct a ; solve_var.
+  Qed.
+
+  Lemma Kclose_k_notin : forall K i k, K \notin Kfv_k (Kclose_k K i k).
+  Proof. intros. induction k ; simpls~. apply~ Kclose_d_notin. Qed.
+
+  Lemma Kclose_ty_notin : forall K i ty, K \notin Kfv_ty (Kclose_ty K i ty).
+  Proof.
+    intros.
+    induction ty ; intros ; solve_var ; rewrite_all notin_union ; try split~.
+    - apply~ Kclose_k_notin.
+    - apply~ Kclose_d_notin.
+  Qed.
 
   Lemma Kclose_t_notin : forall K i t, K \notin Kfv_t (Kclose_t K i t).
-  Proof. Admitted.
+  Proof.
+    intros. gen i.
+    induction t ; intros ; solve_var ; rewrite_all notin_union ; splits~ ;
+      try solve [ apply~ Kclose_d_notin
+                | apply~ Kclose_k_notin
+                | apply~ Kclose_ty_notin ].
+    destruct c ; solve_var.
+  Qed.
 
   Lemma Tsubst_t_open_distr :
     forall i X T t u,
